abstract page table update

Page_Tables/PageTable_seL4.thy
@@ -48,14 +48,20 @@ text \<open>Supported page types\<close>
 
 datatype page_type =
    ArmSmallPage
+ | ArmLargePage
  | ArmSection
+ | ArmSuperSection
 
 
 primrec
   page_bits :: "page_type \<Rightarrow> nat"
 where
  "page_bits ArmSmallPage    = 12" |
- "page_bits ArmSection      = 20" 
+ "page_bits ArmLargePage    = 16" |
+ "page_bits ArmSection      = 20" |
+ "page_bits ArmSuperSection = 24"
+
+
 
 definition
   page_size :: "page_type \<Rightarrow> nat" where
@@ -73,6 +79,10 @@ definition
 
 lemma "map (\<lambda>p. vaddr_offset p 0xFEDCBAAA) [ArmSmallPage, ArmSection] = [0xAAA, 0xCBAAA]"
   by (clarsimp simp: vaddr_offset_def mask_def)
+
+lemma "map (\<lambda>p. vaddr_offset p 0xFEDCBAAA) [ArmSmallPage, ArmLargePage, ArmSection, ArmSuperSection] = [0xAAA, 0xBAAA, 0xCBAAA, 0xDCBAAA]"
+  by (clarsimp simp: vaddr_offset_def mask_def)
+
 
 text \<open>Get the non-offset part of an address for a given page size\<close>
 definition
@@ -110,8 +120,9 @@ datatype pde =
  | ReservedPDE
  (* "the paddr is address of a page table" *)
  | PageTablePDE paddr
- (*- "the paddr is base address of section" *)
+ (* "the paddr is base address of section *)
  | SectionPDE paddr arm_perm_bits
+ | SuperSectionPDE paddr arm_perm_bits
 
 
 definition
@@ -130,10 +141,14 @@ definition
   "decode_pde_section w \<equiv> SectionPDE (Addr (addr_base ArmSection w))
                                      (perm_bits_pde_sections w)"
 
+definition
+  "decode_pde_ssection w \<equiv> SuperSectionPDE (Addr (addr_base ArmSuperSection w))
+                                           (perm_bits_pde_sections w)"
 
 definition
   pt_base_mask :: machine_word where
   "pt_base_mask \<equiv> NOT (mask 9)" (* FIXME TODO: check *again* that this is right *)
+
 definition
   "decode_pde_pt w \<equiv> PageTablePDE (Addr (w AND pt_base_mask))"
 
@@ -145,7 +160,8 @@ definition
   "decode_pde w \<equiv> let pde_type = w AND 0x3
             in
               if pde_type = 1 then (decode_pde_pt w)
-              else if pde_type = 2 then decode_pde_section w
+              else if pde_type = 2 & \<not>(w !! 18) then (decode_pde_section w)
+              else if pde_type = 2 &  (w !! 18) then (decode_pde_ssection w)
               else if pde_type = 3 then ReservedPDE
               else InvalidPDE"
 
@@ -162,7 +178,9 @@ section \<open>Page Table Entry (PTE) Decoding\<close>
 datatype pte =
    InvalidPTE
    (* "the paddr is the page base address" *)
+ | LargePagePTE paddr arm_perm_bits
  | SmallPagePTE paddr arm_perm_bits
+
 
 definition
   perm_bits_pte_small :: "machine_word \<Rightarrow> arm_perm_bits" where
@@ -180,21 +198,37 @@ definition
   "decode_pte_small w \<equiv> SmallPagePTE (Addr (addr_base ArmSmallPage w))
                                      (perm_bits_pte_small w)"
 
-
+definition
+  perm_bits_pte_large :: "machine_word \<Rightarrow> arm_perm_bits" where
+  "perm_bits_pte_large w =
+     \<lparr> arm_p_APX = ucast ((w >> 9) AND 0x1),
+       arm_p_AP  = ucast ((w >> 4) AND 0x3),
+       arm_p_TEX = ucast ((w >> 12) AND 0x7),
+       arm_p_S   = ucast ((w >> 10) AND 0x1),
+       arm_p_XN  = ucast ((w >> 15) AND 0x1),
+       arm_p_C   = ucast ((w >> 3) AND 0x1),
+       arm_p_B   = ucast ((w >> 2) AND 0x1),
+       arm_p_nG  = ucast ((w >> 11) AND 0x1) \<rparr>"
 
 definition
   large_base_mask :: "32 word" where
   "large_base_mask \<equiv> NOT (mask 16)"
 
+definition
+  "decode_pte_large w \<equiv> LargePagePTE (Addr (addr_base ArmLargePage w))
+                                     (perm_bits_pte_large w)"
 
 lemma (* sanity check *)
   "large_base_mask \<equiv> 0xFFFF0000" by (simp add: large_base_mask_def mask_def)
 
 definition
   decode_pte :: "machine_word \<Rightarrow> pte" where
-  "decode_pte w \<equiv> if w AND 3 = 0 
-            then InvalidPTE
-            else decode_pte_small w"
+  "decode_pte w \<equiv> if w AND 3 = 0 then InvalidPTE
+                  else if w !! 1 then decode_pte_small w
+                  else decode_pte_large w"
+
+
+
 
 (* update form Hira: changed Option.map to map_option *)
 definition
@@ -221,6 +255,9 @@ definition
   vaddr_pt_index :: "machine_word \<Rightarrow> machine_word" where
   "vaddr_pt_index w \<equiv> (w >> 12) AND mask 8"
 
+value "(mask 18:: 32 word) << 14"
+
+value "(mask (32-14):: 32 word)"
 
 subsection \<open>Get Frame\<close>
 
@@ -234,7 +271,7 @@ definition
      let 
        pd_idx_offset = ((vaddr_pd_index (addr_val vp)) << 2)
      in
-       decode_heap_pde h (root r+ pd_idx_offset)"
+       decode_heap_pde h (Addr (addr_val root && (mask 18:: 32 word) << 14)   r+ pd_idx_offset)"
 
 text \<open>
   Decode the correct page table entry from a page table at some
@@ -261,8 +298,10 @@ definition
    case_option None
     (\<lambda>pte. case pte 
              of InvalidPTE \<Rightarrow> None
-              | SmallPagePTE base perms \<Rightarrow> Some (base, ArmSmallPage, perms))
+              | SmallPagePTE base perms \<Rightarrow> Some (base, ArmSmallPage, perms)
+              | LargePagePTE base perms \<Rightarrow> Some (base, ArmLargePage, perms))
     (get_pte h pt_base vp)"
+
 
 definition
   lookup_pde :: "heap \<Rightarrow> paddr \<Rightarrow> vaddr \<rightharpoonup> (paddr \<times> page_type \<times> arm_perm_bits)"
@@ -272,9 +311,11 @@ definition
     (\<lambda>pde. case pde 
             of InvalidPDE \<Rightarrow> None
              | ReservedPDE \<Rightarrow> None
+             | SuperSectionPDE base perms \<Rightarrow> Some (base, ArmSuperSection, perms)
              | SectionPDE base perms \<Rightarrow> Some (base, ArmSection, perms)
              | PageTablePDE pt_base \<Rightarrow> lookup_pte h pt_base vp)
     (get_pde h root vp)"
+
 
 
 subsection \<open>Get Page\<close>
@@ -333,15 +374,12 @@ definition
        vp_val = addr_val vp ;
        pd_idx_offset = ((vaddr_pd_index vp_val) << 2) ;
        pt_idx_offset = ((vaddr_pt_index vp_val) << 2) ;
-       pd_touched = set (addr_seq (root r+ pd_idx_offset) 4) ;
+       pd_touched = set (addr_seq (Addr (addr_val root && (mask 18:: 32 word) << 14)  r+ pd_idx_offset) 4) ;
        pt_touched = (\<lambda>pt_base. set (addr_seq (pt_base r+ pt_idx_offset) 4))
      in
-      (case decode_heap_pde h (root r+ pd_idx_offset)
-         of Some pde \<Rightarrow> 
-              (case pde 
-                 of PageTablePDE pt_base \<Rightarrow> pd_touched \<union> pt_touched pt_base
-                  | _ \<Rightarrow> pd_touched)
-          | None \<Rightarrow> {})"
+      (case decode_pde (the (load_machine_word h (Addr (addr_val root && (mask 18:: 32 word) << 14)  r+ pd_idx_offset)))
+            of  PageTablePDE pt_base \<Rightarrow> pd_touched \<union> pt_touched pt_base
+                 | _ \<Rightarrow> pd_touched)"
 
 
 section \<open>Properties, Instantiation to pagetable Locale\<close>
@@ -467,7 +505,7 @@ text \<open>Heap monotonicity of ptable_trace works a bit differently as it just
 (*XXX: fold into not_in_trace_not_in_pde?*)
 lemma lift_valid_pde_valid:
   "\<lbrakk> ptable_lift h r vp = Some p \<rbrakk> 
-   \<Longrightarrow> decode_heap_pde h (r r+ (vaddr_pd_index (addr_val vp) << 2)) \<noteq> None"
+   \<Longrightarrow> decode_heap_pde h (Addr (addr_val r && (mask 18:: 32 word) << 14) r+ (vaddr_pd_index (addr_val vp) << 2)) \<noteq> None"
   unfolding ptable_lift_def lookup_pde_def Let_def get_pde_def
   by (auto split: option.splits)
 
@@ -475,11 +513,12 @@ lemma ptable_trace_heap_mono_simp:
   "\<lbrakk> ptable_lift h r vp = Some p ; h \<bottom> h' \<rbrakk>
    \<Longrightarrow> ptable_trace (h ++ h') r vp = ptable_trace h r vp"
   unfolding ptable_trace_def Let_def
-  apply (case_tac "decode_heap_pde h (r r+ (vaddr_pd_index (addr_val vp) << 2))")
+  apply (case_tac "decode_heap_pde h (Addr (addr_val r && (mask 18:: 32 word) << 14) r+ (vaddr_pd_index (addr_val vp) << 2))")
    apply (drule lift_valid_pde_valid, blast)
-  apply (subst decode_pde_heap_mono_simp, assumption+)
-  apply simp
-  done
+  apply (frule_tac h' =  h' in decode_pde_heap_mono_simp, simp, simp add: decode_heap_pde_def)
+  by auto
+
+
 (*XXX: any set-like monotonicity properties can be derived from this*)
 
 
@@ -528,7 +567,7 @@ lemma lookup_pde_frame_mono_option:
   unfolding frame_mono_option_def lookup_pde_def load_machine_word_def 
             load_value_def Let_def get_pde_def
   apply (intro allI impI, elim conjE)
-  apply (case_tac "decode_heap_pde h (r r+ (vaddr_pd_index (addr_val vp) << 2))")
+  apply (case_tac "decode_heap_pde h (Addr (addr_val r && (mask 18:: 32 word) << 14) r+ (vaddr_pd_index (addr_val vp) << 2))")
    apply simp
   apply simp
   apply (drule (1) decode_pde_heap_mono)
@@ -561,6 +600,9 @@ lemma get_page_frame_mono_option:
 
 lemmas get_page_frame_mono = frame_mono_optionE[OF get_page_frame_mono_option]
 
+(* we have to fix the trace *)
+
+
 
 subsection \<open>Preservation of trace and lift During Updates Outside a Trace\<close>
 
@@ -576,16 +618,28 @@ lemma decode_pte_update_eq:
   unfolding decode_pte_def decode_heap_pte_def load_machine_word_def
   by (simp add: load_value_update_eq)
 
+
+(*lemma  not_in_trace_not_in_pde:
+  "\<lbrakk>p \<notin> ptable_trace h r vp ; ptable_lift h r vp = Some p \<rbrakk> \<Longrightarrow> 
+      p \<notin> set (addr_seq (Addr (addr_val r && (mask 18:: 32 word) << 14)  r+ (vaddr_pd_index (addr_val vp) << 2)) 4)"
+  apply (subgoal_tac "\<exists>pde. 
+         decode_heap_pde h (Addr (addr_val r && (mask 18:: 32 word) << 14)  r+ (vaddr_pd_index (addr_val vp) << 2)) = Some pde")
+   prefer 2
+   apply (fastforce dest: lift_valid_pde_valid)
+  apply (clarsimp simp: ptable_trace_def Let_def decode_heap_pde_def)
+  by (case_tac "decode_pde z"; clarsimp)
+*)
+
 lemma not_in_trace_not_in_pde:
   assumes trace: "p \<notin> ptable_trace h r vp"
   assumes lift: "ptable_lift h r vp = Some p"
-  shows "p \<notin> set (addr_seq (r r+ (vaddr_pd_index (addr_val vp) << 2)) 4)"
+  shows "p \<notin> set (addr_seq (Addr (addr_val r && (mask 18:: 32 word) << 14)  r+ (vaddr_pd_index (addr_val vp) << 2)) 4)"
 proof -
   from lift 
   obtain pde where 
-    "decode_heap_pde h (r r+ (vaddr_pd_index (addr_val vp) << 2)) = Some pde "
+    "decode_heap_pde h (Addr (addr_val r && (mask 18:: 32 word) << 14)  r+ (vaddr_pd_index (addr_val vp) << 2)) = Some pde "
     by (auto dest: lift_valid_pde_valid)
-  thus ?thesis using trace unfolding ptable_trace_def Let_def
+  thus ?thesis using trace unfolding ptable_trace_def Let_def decode_heap_pde_def
     by (cases pde, auto)
 qed
 
@@ -594,8 +648,8 @@ lemma ptable_trace_preserved':
   "\<lbrakk> p \<notin> ptable_trace h r vp ; ptable_lift h r vp = Some p \<rbrakk> 
   \<Longrightarrow> ptable_trace (h(p \<mapsto> v)) r vp = ptable_trace h r vp"
   apply (frule (1) not_in_trace_not_in_pde)
-  apply (unfold ptable_trace_def ptable_lift_def Let_def lookup_pde_def)
-  apply (simp add: decode_pde_update_eq)
+  apply (unfold ptable_trace_def ptable_lift_def Let_def lookup_pde_def )
+  apply (simp add: decode_pde_update_eq load_machine_word_def load_value_update_eq)
   done
 
 (*XXX:name modified to not conflict with instantiation of locale*)
@@ -603,16 +657,26 @@ lemma ptable_lift_preserved':
   "\<lbrakk> p \<notin> ptable_trace h r vp ; ptable_lift h r vp = Some p \<rbrakk>
     \<Longrightarrow> ptable_lift (h(p \<mapsto> v)) r vp = Some p"
   apply (frule (1) not_in_trace_not_in_pde)
-  apply (unfold ptable_trace_def ptable_lift_def lookup_pde_def lookup_pte_def Let_def)
+  apply (unfold ptable_trace_def ptable_lift_def lookup_pde_def lookup_pte_def Let_def get_pde_def )
   apply clarsimp
-  apply (case_tac "decode_heap_pde h (r r+ (vaddr_pd_index (addr_val vp) << 2))")
+  apply (case_tac "decode_heap_pde h (Addr (addr_val r && mask 18 << 14) r+ (vaddr_pd_index (addr_val vp) << 2))")
    apply (simp add: get_pde_def)
   apply (rule_tac x=a and y=aa in exI2)
   apply clarsimp
   apply (rename_tac pde)
-  apply (case_tac pde)
-      apply (clarsimp simp: get_pde_def get_pte_def Let_def 
-                            decode_pde_update_eq decode_pte_update_eq)+
+  apply (rule_tac x=b in exI)
+  apply (case_tac pde; clarsimp)
+    apply (subgoal_tac 
+      "decode_heap_pde (h(a r+ vaddr_offset aa (addr_val vp) \<mapsto> v)) (Addr ((addr_val r && mask 18 << 14) + (vaddr_pd_index (addr_val vp) << 2))) =
+                Some (PageTablePDE x3)")
+     apply clarsimp
+     apply (clarsimp simp: get_pte_def)
+     apply (subgoal_tac " decode_heap_pte (h(a r+ vaddr_offset aa (addr_val vp) \<mapsto> v)) (x3 r+ (vaddr_pt_index (addr_val vp) << 2)) =
+         decode_heap_pte h (x3 r+ (vaddr_pt_index (addr_val vp) << 2)) ")
+      apply clarsimp 
+     apply (rule decode_pte_update_eq)
+     apply (clarsimp simp: decode_heap_pde_def)
+    apply (clarsimp simp:    decode_pde_update_eq )+
   done
   (*XXX: shorter, but still ugly proof*)
 
